language_formalisation/syntax/syntax.v
@@ -24,7 +24,7 @@ Inductive val : Type :=
 with comp : Type :=
 | Ret : val -> comp
 | Absurd : val -> comp
-| ΠMatch : val -> var_name * var_name -> comp -> comp (* x~1 y~0 *)
+| ΠMatch : val -> var_name -> var_name -> comp -> comp (* x~1 y~0 *)
 | ΣMatch : val -> var_name -> comp -> var_name -> comp -> comp
 | App : val -> val -> comp
 | Op : op_id -> val -> var_name -> comp -> comp (* x~1 k~0 *)
@@ -75,14 +75,14 @@ with eqs : Type :=
 
 (* Auxiliary Function Definitions *)
 
-Fixpoint get_vtype (Γ : ctx) (i:nat) : option vtype :=
+Fixpoint get_vtype Γ i :=
   match Γ, i with
   | CtxØ , _=> None
   | CtxU Γ' A, 0 => Some A
   | CtxU Γ' A, S i' =>  get_vtype Γ' i'
   end.
 
-Fixpoint get_ttype (Z : tctx) (i:nat) : option vtype :=
+Fixpoint get_ttype Z i :=
   match Z, i with
   | TCtxØ , _=> None
   | TCtxU Z' A, 0 => Some A
@@ -90,7 +90,7 @@ Fixpoint get_ttype (Z : tctx) (i:nat) : option vtype :=
   end.
 
 
-Fixpoint get_op_type (Σ : sig) (op : op_id) : option (vtype * vtype) :=
+Fixpoint get_op_type Σ op :=
   match Σ with
   | SigØ => None
   | SigU Σ' op' A B =>
@@ -99,8 +99,7 @@ Fixpoint get_op_type (Σ : sig) (op : op_id) : option (vtype * vtype) :=
   end.
 
 
-Fixpoint find_op_case (h : hcases) (op : op_id) 
-  : option (var_name * var_name * comp) :=
+Fixpoint find_op_case h op : option (var_name * var_name * comp) :=
   match h with
   | CasesØ => None
   | CasesU h_others op' x_op k_op c_op =>
@@ -132,7 +131,7 @@ with c_no_var_j (c:comp) (j:nat) :=
 match c with
 | Ret v => v_no_var_j v j
 | Absurd v => v_no_var_j v j 
-| ΠMatch v (x, y) c => 
+| ΠMatch v x y c => 
     (v_no_var_j v j) /\ c_no_var_j c (j+2)
 | ΣMatch v xl cl xr cr =>
     (v_no_var_j v j) /\ (c_no_var_j cl (j+1)) /\ (c_no_var_j cr (j+1))
@@ -147,61 +146,6 @@ match h with
 | CasesØ => True
 | CasesU h op x k c => (h_no_var_j h j) /\ (c_no_var_j c (j+2))
 end.
-
-
-Fixpoint v_switch_vars (v:val) (i:nat) (j:nat) :=
-match v with
-| Var (name, num) =>
-    if num =? i then Var (name, j)
-    else if num =? j then Var (name, i)
-    else Var (name, num)
-| Unit => Unit
-| Int n => Int n
-| Inl v' => Inl (v_switch_vars v' i j)
-| Inr v' => Inr (v_switch_vars v' i j)
-| Pair v1 v2 => Pair (v_switch_vars v1 i j) (v_switch_vars v2 i j)
-| Fun x c => Fun x (c_switch_vars c (i+1) (j+1))
-| Handler x c_ret h =>
-    Handler x (c_switch_vars c_ret (i+1) (j+1)) (h_switch_vars h i j)
-end
-with c_switch_vars (c:comp) (i:nat) (j:nat) :=
-match c with
-| Ret v => Ret (v_switch_vars v i j)
-| Absurd v => Absurd (v_switch_vars v i j)
-| ΠMatch v (x, y) c =>
-    ΠMatch (v_switch_vars v i j) (x,y) (c_switch_vars c (i+2) (j+2))
-| ΣMatch v xl cl xr cr =>
-    ΣMatch (v_switch_vars v i j) xl (c_switch_vars cl (i+1) (j+1)) 
-      xr (c_switch_vars cr (i+1) (j+1))
-| App v1 v2 => App (v_switch_vars v1 i j) (v_switch_vars v2 i j)
-| Op op v_arg y c => 
-    Op op (v_switch_vars v_arg i j) y (c_switch_vars c (i+1) (j+1))
-| LetRec f x c1 c2 =>
-    LetRec f x (c_switch_vars c1 (i+2) (j+2)) (c_switch_vars c2 (i+1) (j+1))
-| DoBind x c1 c2 => 
-    DoBind x (c_switch_vars c1 i j) (c_switch_vars c2 (i+1) (j+1))
-| Handle v c' => Handle (v_switch_vars v i j) (c_switch_vars c' i j)
-end
-with h_switch_vars (h:hcases) (i:nat) (j:nat) :=
-match h with
-| CasesØ => CasesØ
-| CasesU h op x k c =>
-    CasesU (h_switch_vars h i j) op x k (c_switch_vars c (i+2) (j+2))
-end.
-
-
-Fixpoint ctx_change_var (Γ:ctx) (i:nat) (A:vtype) :=
-  match Γ, i with
-  | CtxØ, _ => CtxØ
-  | CtxU Γ' A', 0 => CtxU Γ' A
-  | CtxU Γ' A', S i' => CtxU (ctx_change_var Γ' i' A) A'
-  end.
-
-
-Definition ctx_switch_vars (Γ : ctx) (i:nat) (j:nat) (A:vtype) (B:vtype)
-  (proof_i : get_vtype Γ i = Some A) (proof_j: get_vtype Γ j = Some B) : ctx
-:=
-  ctx_change_var (ctx_change_var Γ i B) j A.
 
 
 Fixpoint ctx_remove_var (Γ:ctx) (i:nat) :=
