language_formalisation/type_system/subtyping.v
@@ -4,39 +4,39 @@ Require Import syntax.
 
 
 Inductive vsubtype : vtype -> vtype -> Prop :=
-| VsubtyUnit : vsubtype TyUnit TyUnit
-| VsubtyInt : vsubtype TyInt TyInt
-| VsubtyTyØ : vsubtype TyØ TyØ
-| VsubtyTyΣ A A' B B' : 
+| SubtypeUnit : vsubtype TyUnit TyUnit
+| SubtypeInt : vsubtype TyInt TyInt
+| SubtypeTyØ : vsubtype TyØ TyØ
+| SubtypeTyΣ A A' B B' : 
     vsubtype A A' -> vsubtype B B' -> vsubtype (TyΣ A B) (TyΣ A' B')
-| VsubtyTyΠ A A' B B' : 
+| SubtypeTyΠ A A' B B' : 
     vsubtype A A' -> vsubtype B B' -> vsubtype (TyΠ A B) (TyΠ A' B')
-| VsubtyFun A A' C C' : 
+| SubtypeTyFun A A' C C' : 
     vsubtype A' A -> csubtype C C' -> vsubtype (TyFun A C) (TyFun A' C')
-| VsubtyHandler C C' D D': 
+| SubtypeTyHandler C C' D D': 
     csubtype C' C -> csubtype D D' -> vsubtype (TyHandler C D) (TyHandler C' D')
 
 with csubtype : ctype -> ctype -> Prop  :=
-| Csubty A A' Σ Σ' E E': 
+| SubtypeCTy A A' Σ Σ' E E': 
     vsubtype A A' -> sig_subtype Σ Σ' -> eqs_subtype E E' ->
     csubtype (CTy A Σ E) (CTy A' Σ' E')
 
 with sig_subtype : sig -> sig -> Prop :=
-| SigØsubty Σ: sig_subtype SigØ Σ
-| SigUsubty Σ Σ' op A B A' B' : 
+| SubtypeSigØ Σ: sig_subtype SigØ Σ
+| SubtypeSigU Σ Σ' op A B A' B' : 
     sig_subtype Σ Σ' -> get_op_type Σ' op = Some (A', B') -> 
     vsubtype A A' -> vsubtype B' B ->
     sig_subtype (SigU Σ op A B) Σ'
 
 with eqs_subtype : eqs -> eqs -> Prop :=
-| EqsØsubty E: eqs_subtype EqsØ E
-| EqsUsubty E E' Γ Z T1 T2 : 
+| SubtypeEqsØ E: eqs_subtype EqsØ E
+| SubtypeEqsU E E' Γ Z T1 T2 : 
     eqs_subtype E E' -> eqs_contain_eq E' Γ Z T1 T2 ->
     eqs_subtype (EqsU E Γ Z T1 T2) E'
 .
 
 Inductive ctx_subtype : ctx -> ctx -> Prop :=
-| CtxØsubty : ctx_subtype CtxØ CtxØ
-| CtxUsubty Γ Γ' A A' : 
+| SubtypeCtxØ : ctx_subtype CtxØ CtxØ
+| SubtypeCtxU Γ Γ' A A' : 
     ctx_subtype Γ Γ' -> vsubtype A A' -> ctx_subtype (CtxU Γ A) (CtxU Γ' A')
 .
