language_formalisation/type_system/subtyping_lemmas.v
@@ -5,7 +5,7 @@ Add LoadPath "C:\Users\Ziga\Documents\Ziga_podatki\PHD\language_formalisation\su
 (* Add LoadPath "E:\Ziga_Podatki\faks\PHD\language_formalisation\type_system". *)
 (* Add LoadPath "E:\Ziga_Podatki\faks\PHD\language_formalisation\substitution". *)
 
-Require Import syntax declarational wellfounded_lemmas.
+Require Import declarational wf_lemmas.
 
 
 Ltac inv H := inversion H; clear H; subst.
@@ -20,37 +20,26 @@ Lemma sig_subtype_gets_Some Σ Σ' op A B :
 Proof.
 intros sty gets. induction sty; simpl in gets. discriminate.
 destruct (op == op0).
-- injection gets. intros. subst. exists A'. exists B'.
-  constructor. assumption. constructor; assumption.
+- inv gets. exists A'. exists B'. auto.
 - apply IHsty in gets. assumption.
-Qed.
-
-
-Lemma sig_subtype_gets_None Σ Σ' op :
-  sig_subtype Σ Σ' -> get_op_type Σ' op = None -> get_op_type Σ op = None.
-Proof.
-intros sty gets. induction sty; simpl. reflexivity.
-destruct (op == op0); auto.
-rewrite e in *. rewrite gets in H. discriminate.
 Qed.
 
 
 Lemma sig_subtype_extend Σ Σ' op A B :
   sig_subtype Σ Σ' -> wf_sig (SigU Σ' op A B) -> sig_subtype Σ (SigU Σ' op A B).
 Proof.
-intros.
-induction H.
-+ apply SigØsubty.
-+ eapply SigUsubty; eauto.
+intros. induction H.
++ apply SubtypeSigØ.
++ eapply SubtypeSigU; eauto.
   inv H0. simpl. destruct (op0 == op). 
   * rewrite e in *. rewrite H1 in H9. discriminate.
-  * exact H1.
+  * assumption.
 Qed.
 
 
-Lemma sig_subtype_sigempty Σ : sig_subtype Σ SigØ -> Σ = SigØ.
+Lemma sig_subtype_empty Σ : sig_subtype Σ SigØ -> Σ = SigØ.
 Proof.
-intro subty. inv subty. reflexivity. simpl in H1. discriminate.
+intro subty. inv subty. reflexivity. simpl in *. discriminate.
 Qed.
 
 
@@ -59,17 +48,18 @@ Lemma eqs_subtype_extend E E' Σ Γ Z T1 T2 :
   eqs_subtype E (EqsU E' Γ Z T1 T2).
 Proof.
 intros. induction H.
-apply EqsØsubty.
-eapply EqsUsubty. auto. simpl. right. assumption.
++ apply SubtypeEqsØ.
++ eapply SubtypeEqsU. auto. simpl. right. assumption.
 Qed.
 
 
 Lemma eqs_subtype_contains E E' Γ Z T1 T2 :
-  eqs_subtype E E' -> eqs_contain_eq E Γ Z T1 T2 -> eqs_contain_eq E' Γ Z T1 T2.
+  eqs_subtype E E' -> eqs_contain_eq E Γ Z T1 T2 -> 
+  eqs_contain_eq E' Γ Z T1 T2.
 Proof.
 intros sty gets. induction sty; simpl in gets; destruct gets.
-- destruct H0 as [a [b [c ]]]. subst. assumption.
-- auto.
++ destruct H0 as [a [b [c ]]]. subst. assumption.
++ auto.
 Qed.
 
 (* ========================== Basic Properties ========================== *)
@@ -81,36 +71,36 @@ with eqs_subtype_refl E Σ : wf_eqs E Σ -> eqs_subtype E E
 with ctx_subtype_refl Γ : wf_ctx Γ -> ctx_subtype Γ Γ.
 Proof.
 {intros; induction v; inv H.
-+ apply VsubtyUnit.
-+ apply VsubtyInt.
-+ apply VsubtyTyØ.
-+ apply VsubtyTyΣ; auto.
-+ apply VsubtyTyΠ; auto.
-+ apply VsubtyFun. apply IHv. assumption. apply csubtype_refl. assumption.
-+ apply VsubtyHandler; apply csubtype_refl; assumption.
-}{ destruct c. intros. inv H. apply Csubty.
++ apply SubtypeUnit.
++ apply SubtypeInt.
++ apply SubtypeTyØ.
++ apply SubtypeTyΣ; auto.
++ apply SubtypeTyΠ; auto.
++ apply SubtypeTyFun. apply IHv. assumption. apply csubtype_refl. assumption.
++ apply SubtypeTyHandler; apply csubtype_refl; assumption.
+}{ destruct c. intros. inv H. apply SubtypeCTy.
 apply vsubtype_refl. assumption. 
 apply sig_subtype_refl. assumption.
-eapply eqs_subtype_refl. exact H5.
+eapply eqs_subtype_refl. eauto.
 }{ 
 intros; induction Σ.
-+ apply SigØsubty.
-+ eapply SigUsubty.
++ apply SubtypeSigØ.
++ eapply SubtypeSigU.
   - apply sig_subtype_extend. apply IHΣ. inv H. assumption. assumption.
   - simpl. destruct (o==o). reflexivity. destruct n. reflexivity.
   - apply vsubtype_refl. inv H. assumption.
   - apply vsubtype_refl. inv H. assumption.
 }{induction E; intros.
-+ apply EqsØsubty.
-+ apply EqsUsubty. inv H. eapply eqs_subtype_extend. 
++ apply SubtypeEqsØ.
++ apply SubtypeEqsU. inv H. eapply eqs_subtype_extend. 
   - apply IHE. assumption.
   - apply WfEqsU; eauto.
   - simpl. left. auto.
 }
 {clear csubtype_refl sig_subtype_refl eqs_subtype_refl ctx_subtype_refl.
 induction Γ; intros.
-apply CtxØsubty.
-apply CtxUsubty; inv H. apply IHΓ. assumption. 
+apply SubtypeCtxØ.
+apply SubtypeCtxU; inv H. apply IHΓ. assumption. 
 apply vsubtype_refl. assumption.
 }
 Qed.
@@ -122,34 +112,32 @@ Fixpoint eqs_subtype_trans E1 E2 E3
   eqs_subtype E2 E3 -> eqs_subtype E1 E3.
 Proof.
 intros E23. destruct E12.
-apply EqsØsubty.
-eapply EqsUsubty.
-+ eapply eqs_subtype_trans. exact E12. all : assumption.
-+ eapply eqs_subtype_contains. exact E23. assumption.
+apply SubtypeEqsØ.
+eapply SubtypeEqsU.
++ eapply eqs_subtype_trans; eauto.
++ eapply eqs_subtype_contains; eauto.
 Qed.
 
 
 (* Weird notation for SPEED! *)
 Fixpoint vsubtype_trans A1 A2 A3 
-  (A12 : vsubtype A1 A2) {struct A12} : vsubtype A2 A3 -> vsubtype A1 A3
-
+  (A12 : vsubtype A1 A2) {struct A12} : vsubtype A2 A3 -> 
+  vsubtype A1 A3
 with vsubtype_trans_rev A1 A2 A3
-  (A21 : vsubtype A2 A1) {struct A21} : vsubtype A3 A2 -> vsubtype A3 A1
-
+  (A21 : vsubtype A2 A1) {struct A21} : vsubtype A3 A2 -> 
+  vsubtype A3 A1
 with csubtype_trans C1 C2 C3
-  (C12 : csubtype C1 C2) {struct C12} : csubtype C2 C3 -> csubtype C1 C3
-
+  (C12 : csubtype C1 C2) {struct C12} : csubtype C2 C3 -> 
+  csubtype C1 C3
 with csubtype_trans_rev C1 C2 C3 
-  (C21 : csubtype C2 C1) {struct C21} : csubtype C3 C2 -> csubtype C3 C1
-
+  (C21 : csubtype C2 C1) {struct C21} : csubtype C3 C2 -> 
+  csubtype C3 C1
 with sig_subtype_trans Σ1 Σ2 Σ3 
   (S12 : sig_subtype Σ1 Σ2) {struct S12} : sig_subtype Σ2 Σ3 -> 
   sig_subtype Σ1 Σ3
-
 with sig_subtype_trans_rev Σ1 Σ2 Σ3
   (S21 : sig_subtype Σ2 Σ1) {struct S21} : sig_subtype Σ3 Σ2 -> 
   sig_subtype Σ3 Σ1
-
 with get_op_trans op A' A B B' Σ1 Σ2 (S12 : sig_subtype Σ1 Σ2) {struct S12} :
   get_op_type Σ1 op = Some (A', B') -> vsubtype A A' -> vsubtype B' B ->
   exists A'' B'', 
@@ -158,49 +146,45 @@ Proof.
 {
 clear sig_subtype_trans sig_subtype_trans_rev get_op_trans.
 intros A23; destruct A12; try assumption; inv A23. 
-+ apply VsubtyTyΣ.
-  - eapply vsubtype_trans. exact A12_1. assumption.
-  - eapply vsubtype_trans. exact A12_2. assumption.
-+ apply VsubtyTyΠ.
-  - eapply vsubtype_trans. exact A12_1. assumption.
-  - eapply vsubtype_trans. exact A12_2. assumption.
-+ apply VsubtyFun.
-  - eapply vsubtype_trans_rev. exact A12. assumption. 
-  - eapply csubtype_trans. exact H. assumption.
-+ apply VsubtyHandler.
-  - eapply csubtype_trans_rev. exact H. assumption. 
-  - eapply csubtype_trans. exact H0. assumption.
++ apply SubtypeTyΣ; eapply vsubtype_trans; eauto.
++ apply SubtypeTyΠ; eapply vsubtype_trans; eauto.
++ apply SubtypeTyFun.
+  - eapply vsubtype_trans_rev; eauto. 
+  - eapply csubtype_trans; eauto.
++ apply SubtypeTyHandler.
+  - eapply csubtype_trans_rev; eauto. 
+  - eapply csubtype_trans; eauto.
 }{
 clear sig_subtype_trans sig_subtype_trans_rev get_op_trans.
 intros A32; destruct A21; try assumption; inv A32. 
-+ apply VsubtyTyΣ; eapply vsubtype_trans_rev; eauto.
-+ apply VsubtyTyΠ; eapply vsubtype_trans_rev; eauto.
-+ apply VsubtyFun.
++ apply SubtypeTyΣ; eapply vsubtype_trans_rev; eauto.
++ apply SubtypeTyΠ; eapply vsubtype_trans_rev; eauto.
++ apply SubtypeTyFun.
   - eapply vsubtype_trans; eauto.
   - eapply csubtype_trans_rev; eauto.
-+ apply VsubtyHandler.
++ apply SubtypeTyHandler.
   - eapply csubtype_trans; eauto.
   - eapply csubtype_trans_rev; eauto.
 }{
 clear vsubtype_trans_rev csubtype_trans csubtype_trans_rev.
 clear sig_subtype_trans_rev get_op_trans.
-intros C23; destruct C12. inv C23. apply Csubty.
+intros C23; destruct C12. inv C23. apply SubtypeCTy.
 - eapply vsubtype_trans; eauto.
 - eapply sig_subtype_trans; eauto.
 - eapply eqs_subtype_trans; eauto.
 }{
 clear vsubtype_trans csubtype_trans csubtype_trans.
 clear sig_subtype_trans get_op_trans.
-intros C32; destruct C21. inv C32. apply Csubty.
+intros C32; destruct C21. inv C32. apply SubtypeCTy.
 - eapply vsubtype_trans_rev; eauto.
 - eapply sig_subtype_trans_rev; eauto.
 - eapply eqs_subtype_trans; eauto.
 }{
 clear csubtype_trans csubtype_trans_rev sig_subtype_trans_rev.
 intros S23. destruct S12.
-apply SigØsubty.
+{ apply SubtypeSigØ. }
 apply (sig_subtype_gets_Some Σ' Σ3) in H as H'.
-destruct H' as [A'' [B'' [g]]]. eapply SigUsubty.
+destruct H' as [A'' [B'' [g]]]. eapply SubtypeSigU.
 2 : exact g. all: try assumption.
 + eapply sig_subtype_trans; eauto.
 + clear sig_subtype_trans vsubtype_trans_rev.
@@ -210,29 +194,26 @@ destruct H' as [A'' [B'' [g]]]. eapply SigUsubty.
 }{
 clear csubtype_trans csubtype_trans_rev sig_subtype_trans.
 intros S32. destruct S21.
-apply sig_subtype_sigempty in S32. subst. apply SigØsubty.
+{ apply sig_subtype_empty in S32. subst. apply SubtypeSigØ. }
 induction Σ3.
-apply SigØsubty.
-inv S32. simpl in H8. destruct (o==op).
-+ injection H8. intros. subst. eapply SigUsubty. auto. eauto.
+{ apply SubtypeSigØ. }
+inv S32. simpl in *. destruct (o==op).
++ inv H8. eapply SubtypeSigU. auto. eauto.
   - eapply vsubtype_trans_rev; eauto.
   - eapply vsubtype_trans; eauto.
 + eapply get_op_trans in H8 as gets'.
   2:exact S21. 2:exact H9. 2:exact H10.
-  destruct gets' as [A'' [B'' [gets' [styA'']]]]. eapply SigUsubty.
-  2: exact gets'. all: try assumption.
-  apply IHΣ3. assumption.
+  destruct gets' as [A'' [B'' [gets' [styA'']]]].
+  eapply SubtypeSigU; eauto.
 }{
 clear csubtype_trans csubtype_trans_rev.
 clear sig_subtype_trans sig_subtype_trans_rev get_op_trans.
 intros. revert H. induction S12; intros gets.
 simpl in gets. discriminate.
-simpl in *. destruct (op==op0).
-+ injection gets. intros. subst.
-  exists A'0. exists B'0. constructor. assumption. constructor.
-  eapply vsubtype_trans_rev. exact H2. assumption.
-  eapply vsubtype_trans. exact H3. assumption.
-+ apply IHS12. assumption.
+simpl in *. destruct (op==op0). 2: auto. inv gets.
+exists A'0. exists B'0. constructor. assumption. constructor.
+- eapply vsubtype_trans_rev; eauto.
+- eapply vsubtype_trans; eauto.
 }
 Qed.
 
@@ -244,9 +225,8 @@ Proof.
 revert num. induction csty. clear ctx_subtype_get.
 + intros num H. simpl in H. discriminate.
 + intros num get. destruct num.
-  - clear IHcsty. simpl in *. injection get. intros. subst. exists A'.
-    constructor. reflexivity. assumption.
-  - simpl in *. eapply IHcsty. exact get.
+  - clear IHcsty. simpl in *. inv get. exists A'. auto.
+  - simpl in *. eapply IHcsty. assumption.
 Qed.
 
 
@@ -257,8 +237,7 @@ Proof.
 revert num. induction csty. clear ctx_subtype_get_rev.
 + intros num H. simpl in H. discriminate.
 + intros num get. destruct num.
-  - clear IHcsty. simpl in *. injection get. intros. subst. exists A0.
-    constructor. reflexivity. assumption.
+  - clear IHcsty. simpl in *. inv get. exists A0. auto.
   - simpl in *. eapply IHcsty. exact get.
 Qed.
 
@@ -277,27 +256,24 @@ intros wf ctxsty.
 destruct types. induction H1; apply TypeV; try assumption.
 + apply TypeUnit.
 + apply TypeInt.
-+ apply (ctx_subtype_get_rev _ _ A num) in ctxsty.
-  destruct ctxsty as [A' [gets]]. 
-  eapply TypeVSubtype.
-  - apply TypeV. assumption. apply ctx_gets_wf in gets as wfA'.
-    exact wfA'. assumption. apply TypeVar. assumption.
-  - assumption.
-  - assumption.
++ apply (ctx_subtype_get_rev _ _ A n) in ctxsty.
+  destruct ctxsty as [A' [gets]]. 2: assumption. 
+  eapply TypeVSubtype. 2: eauto.
+  apply TypeV. assumption. apply ctx_gets_wf in gets as wfA'; eauto.
+  apply TypeVar. assumption.
 + apply TypePair; apply (ctx_subtype_vtype Γ Γ'); assumption.
 + apply TypeInl. apply (ctx_subtype_vtype Γ Γ'); assumption.
 + apply TypeInr. apply (ctx_subtype_vtype Γ Γ'); assumption.
-+ apply TypeFun. eapply ctx_subtype_ctype.
++ apply TypeFun. eapply ctx_subtype_ctype; inv H0.
   - exact H1.
-  - apply WfCtxU. assumption. inv H0. assumption.
-  - apply CtxUsubty. exact ctxsty. apply vsubtype_refl. inv H0. assumption.
-+ apply TypeHandler. eapply ctx_subtype_ctype.
+  - apply WfCtxU; assumption.
+  - apply SubtypeCtxU. assumption. apply vsubtype_refl. assumption.
++ apply TypeHandler. eapply ctx_subtype_ctype; inv H0; inv H5.
   - exact H1.
-  - apply WfCtxU. assumption. inv H0. inv H5. assumption.
-  - apply CtxUsubty. exact ctxsty. apply vsubtype_refl.
-    inv H0. inv H5. assumption.
+  - apply WfCtxU; assumption.
+  - apply SubtypeCtxU. assumption. apply vsubtype_refl. assumption.
   - eapply (ctx_subtype_htype Γ Γ'); assumption.
-+ eapply TypeVSubtype. 2 : exact H2.
++ eapply TypeVSubtype. 2 : eauto.
   eapply (ctx_subtype_vtype Γ Γ'); assumption.
 }{
 intros wf ctxsty.
@@ -306,25 +282,24 @@ destruct types. induction H1; apply TypeC; try assumption.
 + apply TypeAbsurd. eapply (ctx_subtype_vtype Γ Γ'); assumption.
 + eapply TypeΠMatch.
   - eapply (ctx_subtype_vtype Γ Γ'). exact H1. all: assumption.
-  - eapply ctx_subtype_ctype.
-    * exact H2.
-    * inv H2. inv H3. inv H7. apply WfCtxU. apply WfCtxU. all: assumption.
-    * apply CtxUsubty. apply CtxUsubty. exact ctxsty.
-      all: inv H2; inv H3; inv H7; apply vsubtype_refl; assumption.
+  - eapply ctx_subtype_ctype. exact H2. all: inv H2; inv H3; inv H7.
+    * apply WfCtxU. apply WfCtxU. all: assumption.
+    * apply SubtypeCtxU. apply SubtypeCtxU. assumption.
+      all: apply vsubtype_refl; assumption.
 + eapply TypeΣMatch.
-  - eapply ctx_subtype_vtype.  exact H1. all: assumption.
+  - eapply ctx_subtype_vtype. exact H1. all: assumption.
   - eapply ctx_subtype_ctype. exact H2. all: inv H2; inv H4. 
     * apply WfCtxU; assumption.
-    * apply CtxUsubty. exact ctxsty. apply vsubtype_refl. assumption.
+    * apply SubtypeCtxU. exact ctxsty. apply vsubtype_refl. assumption.
   - eapply ctx_subtype_ctype. exact H3. all: inv H3; inv H4. 
     * apply WfCtxU; assumption.
-    * apply CtxUsubty. exact ctxsty. apply vsubtype_refl. assumption.
+    * apply SubtypeCtxU. exact ctxsty. apply vsubtype_refl. assumption.
 + eapply TypeDoBind.
   - eapply ctx_subtype_ctype. exact H1. all: assumption.
   - inv H1. inv H4. eapply ctx_subtype_ctype.
     * exact H2.
     * apply WfCtxU; assumption.
-    * apply CtxUsubty. exact ctxsty. apply vsubtype_refl. assumption.
+    * apply SubtypeCtxU. exact ctxsty. apply vsubtype_refl. assumption.
 + eapply TypeApp.
   - eapply ctx_subtype_vtype. exact H1. all: assumption.
   - eapply ctx_subtype_vtype. exact H2. all: assumption.
@@ -334,16 +309,16 @@ destruct types. induction H1; apply TypeC; try assumption.
 + eapply TypeLetRec.
   - eapply ctx_subtype_ctype. exact H1. all: inv H2; inv H3.
     * apply WfCtxU. apply WfCtxU. assumption. inv H8. exact H6. exact H8.
-    * apply CtxUsubty. apply CtxUsubty. exact ctxsty.
+    * apply SubtypeCtxU. apply SubtypeCtxU. exact ctxsty.
       apply vsubtype_refl. inv H8. assumption. apply vsubtype_refl. assumption.
   - eapply ctx_subtype_ctype. exact H2. all: inv H2; inv H3.
     * apply WfCtxU; assumption.
-    * apply CtxUsubty. exact ctxsty. apply vsubtype_refl. assumption.
+    * apply SubtypeCtxU. exact ctxsty. apply vsubtype_refl. assumption.
 + eapply TypeOp.
   exact H1. eapply ctx_subtype_vtype. exact H2. assumption. assumption.
   eapply ctx_subtype_ctype. exact H3. all: inv H3; inv H4.
   - apply WfCtxU; assumption.
-  - apply CtxUsubty. assumption. apply vsubtype_refl. assumption.
+  - apply SubtypeCtxU. assumption. apply vsubtype_refl. assumption.
 + eapply TypeCSubtype. 2: exact H2.
   eapply ctx_subtype_ctype. exact H1. all: assumption.
 }{
@@ -355,7 +330,7 @@ destruct types. induction H2; apply TypeH; try assumption.
   eapply ctx_subtype_ctype. exact H4.
   all: inv H4; inv H5; inv H9.
   - apply WfCtxU. apply WfCtxU. all: assumption.
-  - apply CtxUsubty. apply CtxUsubty. assumption.
+  - apply SubtypeCtxU. apply SubtypeCtxU. assumption.
     all: apply vsubtype_refl; assumption.
 }
 Qed.
@@ -371,32 +346,28 @@ Qed.
 Fixpoint subty_shape_pair A B C : vsubtype C (TyΠ A B) -> 
   exists A' B', C = (TyΠ A' B') /\ vsubtype A' A /\ vsubtype B' B.
 Proof.
-intro orig. inv orig. exists A0. exists B0.
-constructor. reflexivity. constructor; assumption.
+intro orig. inv orig. exists A0. exists B0. auto.
 Qed.
 
 
 Fixpoint subty_shape_sum A B C : vsubtype C (TyΣ A B) -> 
   exists A' B', C = (TyΣ A' B') /\ vsubtype A' A /\ vsubtype B' B.
 Proof.
-intro orig. inv orig. exists A0. exists B0.
-constructor. reflexivity. constructor; assumption.
+intro orig. inv orig. exists A0. exists B0. auto.
 Qed.
 
 
 Fixpoint subty_shape_fun A B C : vsubtype C (TyFun A B) -> 
   exists A' B', C = (TyFun A' B') /\ vsubtype A A' /\ csubtype B' B.
 Proof.
-intro orig. inv orig. exists A0. exists C0.
-constructor. reflexivity. constructor; assumption.
+intro orig. inv orig. exists A0. exists C0. auto.
 Qed.
 
 
 Fixpoint subty_shape_handler A B C : vsubtype C (TyHandler A B) -> 
   exists A' B', C = (TyHandler A' B') /\ csubtype A A' /\ csubtype B' B.
 Proof.
-intro orig. inv orig. exists C0. exists D.
-constructor. reflexivity. constructor; assumption.
+intro orig. inv orig. exists C0. exists D. auto.
 Qed.
 
 
@@ -404,53 +375,55 @@ Qed.
 
 
 (* Var *)
-Fixpoint shape_var_full Γ v x num A (orig : has_vtype Γ v A) {struct orig} :
-  v = Var (x, num) -> 
-  (exists A', get_vtype Γ num = Some A' /\ vsubtype A' A).
+Fixpoint shape_var_full Γ v x n A (orig : has_vtype Γ v A) {struct orig} :
+  v = Var (x, n) -> 
+  (exists A', get_vtype Γ n = Some A' /\ vsubtype A' A).
 Proof.
 intros same.
 destruct orig. destruct H1; try discriminate.
-+ clear shape_var_full. exists A. injection same. intros. subst.
++ clear shape_var_full.
+  exists A. inv same.
   constructor. assumption. apply vsubtype_refl. assumption.
-+ subst. eapply shape_var_full in H1. 2: reflexivity.
-  destruct H1 as [A'' [gets]]. exists A''. constructor. assumption.
++ subst. eapply shape_var_full in H1. clear shape_var_full. 2: reflexivity.
+  destruct H1 as [A'' [gets]].
+  exists A''. constructor. assumption.
   eapply vsubtype_trans. exact H1. assumption.
 Qed.
 
 
-Lemma shape_var Γ name num A:
-  has_vtype Γ (Var (name, num)) A -> 
-  (exists A', get_vtype Γ num = Some A' /\ vsubtype A' A).
+Lemma shape_var Γ x n A:
+  has_vtype Γ (Var (x, n)) A -> 
+  (exists A', get_vtype Γ n = Some A' /\ vsubtype A' A).
 Proof.
 intro orig.
-apply (shape_var_full _ _ name num A) in orig as shape. 2: reflexivity.
+apply (shape_var_full _ _ x n A) in orig as shape. 2: reflexivity.
 assumption.
 Qed.
 
 
-Lemma shape_var_empty_ctx var_id A:
-  has_vtype CtxØ (Var var_id) A -> False.
+Lemma shape_var_empty_ctx id A:
+  has_vtype CtxØ (Var id) A -> False.
 Proof.
-intro orig. destruct var_id as (name, num).
-apply (shape_var_full _ _ name num A) in orig as shape. 
+intro orig. destruct id as (x, n).
+apply (shape_var_full _ _ x n A) in orig as shape. 
 2: reflexivity. destruct shape as [A'[gets]]. simpl in gets. discriminate.
 Qed.
 
 
 (* Empty *)
 Fixpoint shape_empty_full Γ v A (orig : has_vtype Γ v A) {struct orig} :
-  A = TyØ -> (exists name num, v = Var (name, num)).
+  A = TyØ -> (exists x n, v = Var (x, n)).
 Proof.
 intros samety.
 destruct orig. destruct H1; try discriminate.
-+ clear shape_empty_full. exists name. exists num. reflexivity.
++ clear shape_empty_full. exists x. exists n. reflexivity.
 + subst. apply subty_shape_empty in H2. subst.
   eapply shape_empty_full in H1; auto.
 Qed.
 
 
 Lemma shape_empty Γ v:
-  has_vtype Γ v TyØ -> (exists name num, v = Var (name, num)).
+  has_vtype Γ v TyØ -> (exists x num, v = Var (x, num)).
 Proof.
 intro orig.
 apply (shape_empty_full _ _) in orig as shape; auto.
@@ -460,22 +433,23 @@ Qed.
 (* Pair *)
 Fixpoint shape_pair_full Γ v A B ty (orig : has_vtype Γ v ty) {struct orig} :
   ty = TyΠ A B ->
-  (exists name num, v = Var (name, num)) \/
+  (exists x n, v = Var (x, n)) \/
   (exists v1 v2, v = Pair v1 v2 /\ has_vtype Γ v1 A /\ has_vtype Γ v2 B).
 Proof.
 intros same.
 destruct orig. destruct H1; try discriminate.
-+ clear shape_pair_full. left. exists name. exists num. reflexivity.
-+ clear shape_pair_full. right. exists v1. exists v2. 
-  constructor. reflexivity. injection same. intros. subst. auto. 
++ clear shape_pair_full. left. exists x. exists n. reflexivity.
++ clear shape_pair_full. right.
+  exists v1. exists v2. constructor. reflexivity.
+  inv same. auto. 
 + rewrite same in H2. apply subty_shape_pair in H2. 
   destruct H2 as [A'' [B'' [pity]]]. subst. 
   apply (shape_pair_full _ _ A'' B'') in H1. clear shape_pair_full. 
   2: reflexivity. destruct H1. auto.
-  right. destruct H1 as [v1 [v2]]. exists v1. exists v2.
-  constructor. destruct H1. assumption.
-  constructor; destruct H1; destruct H3; destruct H2;
-  apply TypeV; inv H0; try assumption; eapply TypeVSubtype; eauto.
+  right. destruct H1 as [v1 [v2]].
+  exists v1. exists v2. destruct H1. destruct H2. destruct H3.
+  constructor. assumption. inv H0. constructor;
+  apply TypeV; try assumption; eapply TypeVSubtype; eauto.
 Qed.
 
 
@@ -486,34 +460,33 @@ Proof.
 intro orig.
 apply (shape_pair_full _ _ A B) in orig as shape. 2: reflexivity.
 destruct shape.
-+ destruct H as [name [num]]. discriminate.
-+ destruct H as [v1' [v2' [same]]]. injection same. intros. subst. assumption.
++ destruct H as [x [n]]. discriminate.
++ destruct H as [v1' [v2' [same]]]. inv same. assumption.
 Qed.
 
 
 (* Sum *)
 Fixpoint shape_sum_full Γ v A B ty (orig : has_vtype Γ v ty) {struct orig} :
   ty = TyΣ A B ->
-  (exists name num, v = Var (name, num)) \/
+  (exists x n, v = Var (x, n)) \/
   (exists v1, v = Inl v1 /\ has_vtype Γ v1 A) \/
   (exists v2, v = Inr v2 /\ has_vtype Γ v2 B).
 Proof.
 intros same.
 destruct orig. destruct H1; try discriminate.
-+ clear shape_sum_full. left. exists name. exists num. reflexivity.
++ clear shape_sum_full. left. exists x. exists n. reflexivity.
 + clear shape_sum_full. right. left. exists v. inv same. auto.
 + clear shape_sum_full. right. right. exists v. inv same. auto.
 + rewrite same in H2. apply subty_shape_sum in H2. 
-  destruct H2 as [A'' [B'' [sigty]]]. subst. 
+  destruct H2 as [A'' [B'' [sigty]]]. subst.
+  inv H0. destruct H2. 
   apply (shape_sum_full _ _ A'' B'') in H1. clear shape_sum_full. 
-  2: reflexivity. destruct H1. auto.
-  right. destruct H1.
-  * left. destruct H1. exists x. destruct H1. constructor. assumption.
-    apply TypeV. assumption. inv H0. assumption. destruct H2.
-    eapply TypeVSubtype; eauto.
-  * right. destruct H1. exists x. destruct H1. constructor. assumption.
-    apply TypeV. assumption. inv H0. assumption. destruct H2.
-    eapply TypeVSubtype; eauto.
+  2: reflexivity. destruct H1. auto. right.
+  do 3 destruct H1; subst.
+  * left. exists x. constructor. reflexivity.
+    apply TypeV; try assumption. eapply TypeVSubtype; eauto.
+  * right. exists x. constructor. reflexivity.
+    apply TypeV; try assumption. eapply TypeVSubtype; eauto.
 Qed.
 
 
@@ -523,7 +496,7 @@ Proof.
 intro orig.
 apply (shape_sum_full _ _ A B) in orig as shape. 2: reflexivity.
 destruct shape.
-+ destruct H as [name [num]]. discriminate.
++ destruct H as [x [n]]. discriminate.
 + destruct H; destruct H; destruct H; inv H. auto.
 Qed.
 
@@ -534,7 +507,7 @@ Proof.
 intro orig.
 apply (shape_sum_full _ _ A B) in orig as shape. 2: reflexivity.
 destruct shape.
-+ destruct H as [name [num]]. discriminate.
++ destruct H as [x [n]]. discriminate.
 + destruct H; destruct H; destruct H; inv H. auto.
 Qed.
 
@@ -542,27 +515,28 @@ Qed.
 (* Function *)
 Fixpoint shape_fun_full Γ v A C ty (orig : has_vtype Γ v ty) {struct orig} :
   ty = TyFun A C ->
-  (exists name num, v = Var (name, num)) \/
+  (exists x n, v = Var (x, n)) \/
   (exists x c, v = Fun x c /\ has_ctype (CtxU Γ A) c C).
 Proof.
 intros same.
 destruct orig. destruct H1; try discriminate.
-+ clear shape_fun_full. left. exists name. exists num. reflexivity.
-+ clear shape_fun_full. right. exists x. exists c. constructor. reflexivity.
-  inv same. assumption.
++ clear shape_fun_full. left. exists x. exists n. reflexivity.
++ clear shape_fun_full. right. inv same. 
+  exists x. exists c. auto.
 + rewrite same in H2. apply subty_shape_fun in H2. 
   destruct H2 as [A'' [C'' [funty]]]. subst. 
   apply (shape_fun_full _ _ A'' C'') in H1. clear shape_fun_full. 
   2: reflexivity. destruct H1. auto.
-  right. destruct H1. destruct H1 as [c']. exists x. exists c'.
+  right. destruct H1. destruct H1 as [c']. 
+  exists x. exists c'.
   destruct H1. constructor. assumption.
   apply TypeC; inv H0.
   * apply WfCtxU; assumption.
   * assumption.
-  * destruct H2. eapply TypeCSubtype. 2: exact H1.
-    eapply ctx_subtype_ctype. exact H3.
+  * destruct H2. eapply TypeCSubtype. 2: eauto.
+    eapply ctx_subtype_ctype. eauto.
     apply WfCtxU; assumption.
-    apply CtxUsubty. apply ctx_subtype_refl. assumption. assumption.
+    apply SubtypeCtxU. apply ctx_subtype_refl. all: assumption.
 Qed.
 
 Lemma shape_fun Γ x c A C :
@@ -571,7 +545,7 @@ Proof.
 intro orig.
 apply (shape_fun_full _ _ A C) in orig as shape. 2: reflexivity.
 destruct shape.
-+ destruct H as [name [num]]. discriminate.
++ destruct H as [y [n]]. discriminate.
 + do 3 (destruct H). inv H. inv H0. apply TypeC; assumption.
 Qed.
 
@@ -579,17 +553,18 @@ Qed.
 Fixpoint shape_handler_full Γ v A Σ E D ty
   (orig : has_vtype Γ v ty) {struct orig} :
   ty = TyHandler (CTy A Σ E) D ->
-  (exists name num, v = Var (name, num)) \/
+  (exists x n, v = Var (x, n)) \/
   (exists x c_r h Σ' D', v = Handler x c_r h /\ 
     has_ctype (CtxU Γ A) c_r D' /\ has_htype Γ h Σ' D'
     /\ sig_subtype Σ Σ' /\ csubtype D' D).
 Proof.
 intros same.
 destruct orig. destruct H1; try discriminate.
-+ clear shape_handler_full. left. exists name. exists num. reflexivity.
++ clear shape_handler_full. left. exists x. exists n. reflexivity.
 + clear shape_handler_full. right.
-  exists x. exists c_ret. exists h. exists Σ. exists D.      
-  constructor. reflexivity. inv same. constructor. assumption.
+  exists x. exists c_ret. exists h. exists Σ. exists D.
+  inv same.      
+  constructor. reflexivity. constructor. assumption.
   constructor. assumption. constructor; inv H2.
   apply sig_subtype_refl. assumption. apply csubtype_refl. assumption.
 + rewrite same in *. apply subty_shape_handler in H2. 
@@ -602,7 +577,7 @@ destruct orig. destruct H1; try discriminate.
   constructor. assumption. destruct H1. constructor.
   - eapply ctx_subtype_ctype. eauto.
     inv H0. inv H7. apply WfCtxU; assumption.
-    apply CtxUsubty. apply ctx_subtype_refl. assumption.
+    apply SubtypeCtxU. apply ctx_subtype_refl. assumption.
     inv H2. assumption.
   - destruct H4 as [tys[sty]]. inv H2. constructor. assumption. constructor.
     eapply sig_subtype_trans; eauto. eapply csubtype_trans; eauto.
@@ -616,8 +591,8 @@ Proof.
 intro orig.
 apply (shape_handler_full _ _ A Σ E D) in orig as shape. 2: reflexivity.
 destruct shape.
-+ destruct H as [name [num]]. discriminate.
-+ do 6 (destruct H). exists x3. exists x4. injection H. intros. subst. auto.
++ destruct H as [y [n]]. discriminate.
++ do 6 (destruct H). exists x3. exists x4. inv H. auto.
 Qed.
 
 (* ========================= Handler Cases Shapes ========================= *)
@@ -643,7 +618,7 @@ revert Σ. induction h; intros Σ tys gets finds.
 simpl in finds. discriminate.
 simpl in *. destruct (op==o).
 - inv tys. inv H2. simpl in *. destruct (o==o). 2: (destruct n; reflexivity).
-  injection finds. injection gets. intros. subst. assumption.
+  inv finds. inv gets. intros. subst. assumption.
 - inv tys. inv H2. eapply IHh; eauto.
   clear IHh. simpl in gets. destruct (op==o).
   * rewrite e in n. destruct n. reflexivity.
@@ -695,14 +670,13 @@ Qed.
 (* ΠMatch *)
 Fixpoint shape_prodmatch_full Γ c v x y c' C
   (orig : has_ctype Γ c C) {struct orig} :
-  c = (ΠMatch v (x, y) c') ->
+  c = (ΠMatch v x y c') ->
   (exists A B, has_vtype Γ v (TyΠ A B) /\ has_ctype (CtxU (CtxU Γ A) B) c' C).
 Proof.  
-intros same. destruct orig. destruct H1; try discriminate.
-+ clear shape_prodmatch_full. 
-  inv same. exists A. exists B. auto.
+intros same. destruct orig. destruct H1; try discriminate; inv same.
++ clear shape_prodmatch_full. exists A. exists B. auto.
 + apply (shape_prodmatch_full _ _ v x y c') in H1; clear shape_prodmatch_full. 
-  2: assumption. destruct H1 as [A' [B' [vty]]].
+  2: reflexivity. destruct H1 as [A' [B' [vty]]].
   exists A'. exists B'. constructor. assumption.
   apply TypeC.
   - inv H1. assumption.
@@ -712,7 +686,7 @@ Qed.
 
 
 Fixpoint shape_prodmatch Γ v x y c C :
-  has_ctype Γ (ΠMatch v (x, y) c) C ->
+  has_ctype Γ (ΠMatch v x y c) C ->
   (exists A B, has_vtype Γ v (TyΠ A B) /\  has_ctype (CtxU (CtxU Γ A) B) c C).
 Proof.
 intro orig. apply (shape_prodmatch_full _ _ v x y c) in orig; auto.
@@ -748,6 +722,7 @@ Proof.
 intro orig. apply (shape_summatch_full _ _ v xl cl xr cr) in orig; auto.
 Qed.
 
+
 (* App *)
 Fixpoint shape_app_full Γ c v1 v2 C (orig : has_ctype Γ c C) {struct orig} :
   c = (App v1 v2) ->
@@ -761,9 +736,9 @@ intros same. destruct orig. destruct H1; try discriminate.
   exists A'. constructor. 2: assumption.
   apply TypeV. 
   - assumption.
-  - inv fty. inv H4. apply WfFun; assumption.
-  - eapply TypeVSubtype. exact fty. apply VsubtyFun.
-    apply vsubtype_refl. inv fty. inv H4. assumption. assumption.
+  - inv fty. inv H4. apply WfTyFun; assumption.
+  - eapply TypeVSubtype. exact fty. apply SubtypeTyFun.
+    apply vsubtype_refl. inv fty. inv H4. all: assumption.
 Qed.
 
 
@@ -776,6 +751,7 @@ intro orig. eapply (shape_app_full _ _ (Fun x c) v C) in orig.
 exists A. constructor. apply shape_fun in fty. all: assumption.
 Qed.
 
+
 (* Handle *)
 Fixpoint shape_handle_full Γ c v c' C (orig : has_ctype Γ c C) {struct orig} :
   c = (Handle v c') ->
@@ -787,9 +763,9 @@ intros same. destruct orig. destruct H1; try discriminate.
   clear shape_handle_full. 2: assumption.
   destruct H1 as [D [vty]].
   exists D. constructor. 2: assumption. inv H1.
-  apply TypeV. assumption. apply WfHandler; auto.
+  apply TypeV. assumption. apply WfTyHandler; auto.
   eapply TypeVSubtype. exact vty.
-  apply VsubtyHandler. apply csubtype_refl. all: assumption.
+  apply SubtypeTyHandler. apply csubtype_refl. all: assumption.
 Qed.
 
 Fixpoint shape_handle Γ v c D :
@@ -811,10 +787,10 @@ intros same. destruct orig. destruct H1; try discriminate.
 + clear shape_letrec_full. inv same. exists A. exists C. auto.
 + apply (shape_letrec_full _ _ f x c1 c2) in H1;
   clear shape_letrec_full. 2: assumption.
-  destruct H1 as [A' [C'' [cty]]].
+  destruct H1 as [A' [C'' [cty]]]. inv H1.
   exists A'. exists C''. constructor. assumption.
-  inv H1. apply TypeC; auto.
-  eapply TypeCSubtype. 2: exact H2. apply TypeC; assumption.
+  apply TypeC; auto.
+  eapply TypeCSubtype. 2: eauto. apply TypeC; assumption.
 Qed.
 
 
@@ -840,9 +816,9 @@ intros same samety. destruct orig. destruct H1; try discriminate; inv same.
   clear shape_dobind_full; auto. destruct H1 as [A'' [cty]].
   exists A''. constructor.
   - apply TypeC. assumption. inv cty. inv H0. inv H4.
-    apply WfCty; assumption. eapply TypeCSubtype. exact cty.
+    apply WfCTy; assumption. eapply TypeCSubtype. exact cty.
      inv H2. inv cty. inv H3. 
-    apply Csubty. apply vsubtype_refl. all: assumption.
+    apply SubtypeCTy. apply vsubtype_refl. all: assumption.
   - apply TypeC. inv H1. assumption. assumption.
     eapply TypeCSubtype; eauto.
 Qed.
@@ -868,21 +844,20 @@ intros same samety. destruct orig. destruct H1; try discriminate; inv same.
 + inv samety. clear shape_op_full. exists A_op. exists B_op. auto.
 + destruct C as (A', Σ', E').
   apply (shape_op_full _ _ (CTy A' Σ' E') op v y c' A' Σ' E') in H1;
-  clear shape_op_full. 2: reflexivity. 2: reflexivity.
-  destruct H1 as [A'' [B'' [g [vty]]]]. 
-  inv H2. eapply sig_subtype_gets_Some in g. 2: exact H10.
+  clear shape_op_full; try reflexivity.
+  destruct H1 as [A'' [B'' [g [vty]]]]. inv H2.
+  eapply sig_subtype_gets_Some in g. 2: exact H10.
   destruct g as [A''' [B''' [g' [sty']]]].
   exists A'''. exists B'''.
   constructor. assumption. constructor.
   - apply TypeV. assumption. apply get_op_type_wf in g'. destruct g'.
-    assumption. inv H0. assumption. eapply TypeVSubtype.
-    exact vty. assumption.
+    assumption. inv H0. assumption. eapply TypeVSubtype; eauto.
   - eapply (ctx_subtype_ctype (CtxU Γ B'') (CtxU Γ B''')).
     * apply TypeC. inv H1. assumption. assumption.
-      eapply TypeCSubtype. exact H1. apply Csubty; assumption.
+      eapply TypeCSubtype. exact H1. apply SubtypeCTy; assumption.
     * apply WfCtxU. assumption. apply get_op_type_wf in g'. destruct g'.
       all: inv H0; assumption.
-    * apply CtxUsubty. apply ctx_subtype_refl. all: assumption.
+    * apply SubtypeCtxU. apply ctx_subtype_refl. all: assumption.
 Qed.
 
 
@@ -907,12 +882,12 @@ intros orig. revert Γ'. induction orig; intros Γ' sty cty wfs wfc.
 + eapply WfTApp. eapply ctx_subtype_vtype; eauto. assumption.
 + eapply WfTAbsurd. eapply ctx_subtype_vtype; eauto.
 + eapply WfTΠMatch. eapply ctx_subtype_vtype; eauto. inv H. inv H1.
-  apply IHorig; auto. apply CtxUsubty. 
-  apply CtxUsubty. 4: apply WfCtxU. 4: apply WfCtxU. all: auto.
+  apply IHorig; auto. apply SubtypeCtxU. 
+  apply SubtypeCtxU. 4: apply WfCtxU. 4: apply WfCtxU. all: auto.
   all: apply vsubtype_refl; auto.
 + eapply WfTΣMatch. eapply ctx_subtype_vtype; eauto.  all: inv H; inv H1.
   apply IHorig1; auto. 3: apply IHorig2; auto.
-  1: apply CtxUsubty. 4: apply CtxUsubty.
+  1: apply SubtypeCtxU. 4: apply SubtypeCtxU.
   3: apply WfCtxU. 7: apply WfCtxU. all: auto.
   all: apply vsubtype_refl; auto.
 + eapply sig_subtype_gets_Some in H. 2: exact sty.
@@ -923,7 +898,7 @@ intros orig. revert Γ'. induction orig; intros Γ' sty cty wfs wfc.
     * apply get_op_type_wf in gets'. inv gets'. all: assumption.
     * eapply TypeVSubtype; eauto.
   - apply IHorig; auto.
-    * apply CtxUsubty; auto.
+    * apply SubtypeCtxU; auto.
     * apply get_op_type_wf in gets'. inv gets'. apply WfCtxU. all: assumption.
 Qed.
 
