language_formalisation/substitution/substitution_lemmas.v
@@ -1,0 +1,140 @@
+Add LoadPath "C:\Users\Ziga\Documents\Ziga_podatki\PHD\language_formalisation\substitution".
+Add LoadPath "C:\Users\Ziga\Documents\Ziga_podatki\PHD\language_formalisation\syntax".
+(* Add LoadPath "E:\Ziga_Podatki\faks\PHD\language_formalisation\substitution". *)
+(* Add LoadPath "E:\Ziga_Podatki\faks\PHD\language_formalisation\syntax". *)
+Require Export substitution syntax_lemmas.
+Require Import Arith Le PeanoNat.
+
+
+Lemma v_shift_shift n m cut (v:val) :
+  Sub.v_shift (Sub.v_shift v n cut) m cut = (Sub.v_shift v (n + m) cut)
+
+with c_shift_shift n m cut (c:comp) :
+  Sub.c_shift (Sub.c_shift c n cut) m cut = (Sub.c_shift c (n + m) cut)
+
+with h_shift_shift n m cut (h:hcases) :
+  Sub.h_shift (Sub.h_shift h n cut) m cut = (Sub.h_shift h (n + m) cut).
+Proof.
+{
+clear v_shift_shift.
+revert cut. induction v; intros cut; simpl; f_equal.
+{ (* The only relevant case. *)
+  destruct v as (name, db_i).
+  destruct (cut <=? db_i) eqn:cmp; simpl.
+  - apply (leb_complete _ _) in cmp.
+    assert (cut <= db_i + n) by omega.
+    apply leb_correct in H. rewrite H.
+    f_equal. f_equal. omega.
+  - rewrite cmp. reflexivity. }
+all : try reflexivity || apply IHv || apply IHv1 || apply IHv2.
+all : try apply c_shift_shift || apply h_shift_shift; assumption.
+}{
+clear c_shift_shift.
+revert cut. induction c; intros cut; try destruct p; simpl; f_equal;
+try apply v_shift_shift || apply IHc || apply IHc1 || apply IHc2.
+}{
+clear h_shift_shift.
+revert cut. induction h; intros cut; simpl; f_equal.
+reflexivity. apply IHh. apply c_shift_shift.
+}
+Qed.
+
+Lemma v_shift_makes_no_var v j:
+  v_no_var_j (Sub.v_shift v 1 j) j
+with c_shift_makes_no_var c j:
+  c_no_var_j (Sub.c_shift c 1 j) j
+with h_shift_makes_no_var h j:
+  h_no_var_j (Sub.h_shift h 1 j) j.
+Proof.
+{
+clear v_shift_makes_no_var.
+revert j; induction v; intros j; simpl; auto.
+destruct v as (name, num). simpl.
+destruct (j<=?num) eqn:cmp; simpl.
++ apply leb_complete in cmp. omega.
++ apply leb_iff_conv in cmp. omega.
+}{
+revert j; induction c; intros j; try destruct p; simpl; auto.
+}{
+revert j; induction h; intros j; simpl; auto.
+}
+Qed.
+
+Lemma v_no_var_shift (v:val) j cut:
+  v_no_var_j v j -> (cut <= j) -> v_no_var_j (Sub.v_shift v 1 cut) (j+1)
+
+with c_no_var_shift (c:comp) j cut:
+  c_no_var_j c j -> (cut <= j) -> c_no_var_j (Sub.c_shift c 1 cut) (j+1)
+  
+with h_no_var_shift (h:hcases) j cut:
+  h_no_var_j h j -> (cut <= j) -> h_no_var_j (Sub.h_shift h 1 cut) (j+1).
+Proof.
+{
+clear v_no_var_shift.
+revert j. induction v; intros j orig_clean j_le_cut; simpl; simpl in orig_clean;
+try constructor; try inv orig_clean; auto.
++ destruct v as (name, num). destruct (cut <=? num) eqn:cmp; simpl;
+  try rewrite leb_iff_conv in cmp; omega.
++ apply c_no_var_shift. assumption. omega. 
++ apply c_no_var_shift. assumption. omega.
+}{
+clear c_no_var_shift.
+revert j cut. induction c; intros j cut orig_clean j_le_cut; simpl; simpl in *; 
+try destruct p; try inv orig_clean; try constructor; try constructor; auto;
+try apply IHc || apply IHc1 || apply IHc2; try omega; auto.
++ assert (j+1+2=j+2+1) by omega. rewrite H1. apply IHc. assumption. omega.
++ inv H0. assumption.
++ inv H0. assumption.
++ assert (j+1+2=j+2+1) by omega. rewrite H1. apply IHc1. assumption. omega.
+}{
+clear h_no_var_shift.
+revert j cut. induction h; intros j cut orig_clean j_le_cut; simpl;
+destruct orig_clean; auto. constructor. auto.
+assert (j+1+2=j+2+1) by omega. rewrite H1.
+apply c_no_var_shift. assumption. omega.
+}
+Qed.
+
+
+Lemma v_no_var_sub (v:val) j v_s :
+  v_no_var_j v_s j -> v_no_var_j (Sub.v_sub v (j, v_s)) j
+
+with c_no_var_sub (c:comp) j v_s :
+  v_no_var_j v_s j -> c_no_var_j (Sub.c_sub c (j, v_s)) j
+
+with h_no_var_sub (h:hcases) j v_s :
+  v_no_var_j v_s j -> h_no_var_j (Sub.h_sub h (j, v_s)) j.
+Proof.
+{
+clear v_no_var_sub.
+revert j. induction v; intros j v_s_clean; simpl; try constructor;
+try (apply IHv; assumption); auto.
+- destruct v as (x, n). simpl.
+  induction (n =? j) eqn:fits.
+  + assumption.
+  + simpl. apply Nat.eqb_neq in fits. omega.
+- apply c_no_var_sub. apply v_no_var_shift. assumption. omega.
+- apply c_no_var_sub. apply v_no_var_shift. assumption. omega.
+}{
+clear c_no_var_sub.
+revert j v_s. induction c; intros j v_s v_s_clean; simpl; try constructor;
+try destruct p; simpl; try constructor; auto;
+try apply IHc || apply IHc1 || apply IHc2;
+try (apply v_no_var_shift; assumption || omega).
+all:
+assert (v_no_var_j (Sub.v_shift v_s 1 0) (j + 1)) by
+  (apply v_no_var_shift; auto || omega);
+apply (v_no_var_shift _ _ 0) in H; try omega;
+simpl in H; rewrite v_shift_shift in H; simpl in H;
+assert (j+1+1=j+2) by omega; rewrite H0 in H; assumption.
+}{
+clear h_no_var_sub.
+revert j v_s. induction h; intros j v_s v_s_clean; simpl; auto.
+constructor. auto.
+assert (v_no_var_j (Sub.v_shift v_s 1 0) (j + 1)).
+{ apply v_no_var_shift. auto. omega. }
+apply (v_no_var_shift _ _ 0) in H. simpl in H.
+rewrite (v_shift_shift _ _ _) in H.
+assert (j+1+1=j+2) by omega. rewrite H0 in H. auto. omega.
+}
+Qed.
