language_formalisation/syntax/syntax_lemmas.v
@@ -5,245 +5,6 @@ Require Import Le Compare_dec.
 
 Ltac inv H := inversion H; clear H; subst.
 
-Lemma change_j_get_k Γ j k Aj :
-  j <> k -> get_vtype Γ k = get_vtype (ctx_change_var Γ j Aj) k.
-Proof.
-revert j k. induction Γ; intros j k neq_jk; auto.
-destruct k; destruct j; auto.
-+ omega.
-+ simpl. apply IHΓ. omega.
-Qed.
-
-Lemma change_j_get_j Γ j Aj_orig Aj 
-  (p_j : get_vtype Γ j = Some Aj_orig) :
-  get_vtype (ctx_change_var Γ j Aj) j = Some Aj.
-Proof.
-revert j p_j. induction Γ; intros j p_j; simpl in p_j.
-+ discriminate.
-+ destruct j; auto. simpl. apply IHΓ. assumption.
-Qed.
-
-
-Lemma v_switch_ii v i : v_switch_vars v i i = v
-with c_switch_ii c i : c_switch_vars c i i = c
-with h_switch_ii h i : h_switch_vars h i i = h.
-Proof.
-{
-revert i. induction v; intros i; simpl; try reflexivity;
-try f_equal; try apply IHv || apply IHv1 || apply IHv2.
-+ destruct v as (name, num). destruct (num=?i) eqn:cmp.
-  apply Nat.eqb_eq in cmp. rewrite cmp. reflexivity. reflexivity.
-+ apply c_switch_ii.
-+ apply c_switch_ii.
-+ apply h_switch_ii.
-}{
-revert i. induction c; intros i; simpl; try reflexivity; try destruct p;
-try f_equal; try apply v_switch_ii; try apply IHc || apply IHc1 || apply IHc2.
-}{
-revert i. induction h; intros i; simpl; try reflexivity.
-f_equal. apply IHh. apply c_switch_ii.
-}
-Qed.
-
-Lemma v_switchswitch v i j:
-  v_switch_vars (v_switch_vars v i j) i j = v
-with c_switchswitch c i j:
-  c_switch_vars (c_switch_vars c i j) i j = c
-with h_switchswitch h i j:
-  h_switch_vars (h_switch_vars h i j) i j = h.
-Proof.
-all: revert i j.
-{
-induction v; intros i j; simpl; try reflexivity; try f_equal;
-try apply IHv || apply IHv1 || apply IHv2;
-try apply c_switchswitch || apply h_switchswitch.
-
-destruct v as (name, num).
-destruct (num=?i) eqn:cmpi;
-destruct (num=?j) eqn:cmpj; simpl.
-+ apply Nat.eqb_eq in cmpi. apply Nat.eqb_eq in cmpj. rewrite cmpi in *.
-  rewrite cmpj. rewrite <-beq_nat_refl. auto.
-+ apply Nat.eqb_eq in cmpi. rewrite cmpi in *. rewrite Nat.eqb_neq in cmpj.
-  apply not_eq_sym in cmpj. rewrite <-Nat.eqb_neq in cmpj.
-  rewrite cmpj. rewrite <-beq_nat_refl. reflexivity.
-+ apply Nat.eqb_eq in cmpj. rewrite cmpj in *. rewrite Nat.eqb_neq in cmpi.
-  apply not_eq_sym in cmpi. rewrite <-Nat.eqb_neq in cmpi.
-  rewrite cmpi. rewrite <-beq_nat_refl. reflexivity.
-+ rewrite cmpi. rewrite cmpj. reflexivity.
-}{
-induction c; intros i j; try destruct p; simpl; f_equal;
-try apply v_switchswitch || apply IHc || apply IHc1 || apply IHc2.
-}{
-induction h; intros i j; simpl.
-reflexivity. f_equal. apply IHh. apply c_switchswitch.
-}
-Qed.
-
-Lemma v_switch_sym v i j :
-  v_switch_vars v i j = v_switch_vars v j i
-with c_switch_sym c i j :
-  c_switch_vars c i j = c_switch_vars c j i
-with h_switch_sym h i j :
-  h_switch_vars h i j = h_switch_vars h j i.
-Proof.
-{
-induction v; simpl;
-try f_equal; try apply IHv || apply IHv1 || apply IHv2;
-try apply h_switch_sym || apply c_switch_sym; try reflexivity.
-destruct v as (name, num).
-destruct (num=?i) eqn:cmpi. destruct (num=?j) eqn:cmpj.
-apply Nat.eqb_eq in cmpi. apply Nat.eqb_eq in cmpj.
-rewrite cmpj, cmpi in *. all: auto.
-}{
-revert i j. induction c; intros i j; try destruct p; simpl;
-try f_equal; try apply IHc || apply IHc1 || apply IHc2;
-apply v_switch_sym.
-}{
-induction h; simpl; f_equal; try auto || apply IHh.
-}
-Qed.
-
-Lemma switch_ij_get_k Γ k i j Ai Aj
-  (p_i : get_vtype Γ i = Some Ai) (p_j : get_vtype Γ j = Some Aj) :
-  i <> k -> j <> k ->
-  get_vtype Γ k = get_vtype (ctx_switch_vars Γ i j Ai Aj p_i p_j) k.
-Proof.
-revert k i j p_i p_j. induction Γ;
-intros k i j p_i p_j neq_ik neq_jk. auto.
-revert i j p_i p_j neq_ik neq_jk. destruct k;
-intros i j p_i p_j neq_ik neq_jk.
-+ destruct i.
-  - omega.
-  - simpl. destruct j; auto. omega.
-+ destruct i; destruct j; simpl; auto.
-  - apply change_j_get_k. omega.
-  - apply change_j_get_k. omega.
-  - unfold ctx_switch_vars in IHΓ. apply IHΓ; auto; omega.
-Qed.
-      
-Lemma switch_ij_get_j Γ i j Ai Aj
-  (p_i : get_vtype Γ i = Some Ai) (p_j : get_vtype Γ j = Some Aj) :
-  get_vtype Γ i = get_vtype (ctx_switch_vars Γ i j Ai Aj p_i p_j) j.
-Proof.
-revert i j p_i p_j. induction Γ; intros i j p_i p_j.
-auto.
-destruct i; destruct j; auto; simpl.
-+ apply eq_sym. simpl in p_i. rewrite p_i.
-  apply (change_j_get_j Γ j Aj). auto.
-+ unfold ctx_switch_vars in IHΓ. apply IHΓ. auto. auto.
-Qed.
-
-Lemma switch_ij_get_i Γ i j Ai Aj
-  (p_i : get_vtype Γ i = Some Ai) (p_j : get_vtype Γ j = Some Aj) :
-  get_vtype Γ j = get_vtype (ctx_switch_vars Γ i j Ai Aj p_i p_j) i.
-Proof.
-revert i j p_i p_j. induction Γ; intros i j p_i p_j.
-auto.
-destruct i; destruct j; auto; simpl.
-+ apply eq_sym. simpl in p_j. rewrite p_j.
-  apply (change_j_get_j Γ i Ai). auto.
-+ unfold ctx_switch_vars in IHΓ. apply IHΓ. auto. auto.
-Qed.
-
-Lemma ctx_switch_extend1 Γ A i j Ai Aj
-    (p_i : get_vtype Γ i = Some Ai) (p_j : get_vtype Γ j = Some Aj) 
-    (pp_i : get_vtype (CtxU Γ A) (i+1) = Some Ai)
-    (pp_j : get_vtype (CtxU Γ A) (j+1) = Some Aj) :
-  CtxU (ctx_switch_vars Γ i j Ai Aj p_i p_j) A
-    = 
-  (ctx_switch_vars (CtxU Γ A) (i+1) (j+1) Ai Aj pp_i pp_j).
-Proof.
-revert i j p_i p_j pp_i pp_j. induction Γ; intros i j p_i p_j pp_i pp_j.
-+ destruct i; destruct j; auto.
-+ rename v into G. unfold ctx_switch_vars.
-  assert (forall Γ',
-    CtxU (ctx_change_var Γ' j Ai) A
-      =
-    ctx_change_var (CtxU Γ' A) (j + 1) Ai).
-  * intro. simpl. destruct i; auto; simpl;
-    assert (j+1 = S j) by omega; rewrite H; auto.
-  * specialize (H (ctx_change_var (CtxU Γ G) i Aj)).
-    rewrite H. f_equal.
-    destruct i; auto; simpl.
-    assert (i+1 = S i) by omega; rewrite H0; auto.
-Qed.
-
-Lemma ctx_switch_extend2 Γ B A i j Ai Aj
-    (p_i : get_vtype Γ i = Some Ai) (p_j : get_vtype Γ j = Some Aj) 
-    (pp_i : get_vtype (CtxU (CtxU Γ B) A) (i+2) = Some Ai)
-    (pp_j : get_vtype (CtxU (CtxU Γ B) A) (j+2) = Some Aj) :
-  CtxU (CtxU (ctx_switch_vars Γ i j Ai Aj p_i p_j) B) A
-    = 
-  (ctx_switch_vars (CtxU (CtxU Γ B) A) (i+2) (j+2) Ai Aj pp_i pp_j).
-Proof.
-revert i j p_i p_j pp_i pp_j. induction Γ; intros i j p_i p_j pp_i pp_j.
-+ destruct i; destruct j; simpl in *; discriminate.
-+ rename v into G. unfold ctx_switch_vars.
-  assert (forall Γ',
-    CtxU (CtxU (ctx_change_var Γ' j Ai) B) A
-      =
-    ctx_change_var (CtxU (CtxU Γ' B) A) (j + 2) Ai).
-  * intro. simpl. destruct i; auto; simpl;
-    assert (j+2 = S (S j)) by omega; rewrite H; auto.
-  * specialize (H (ctx_change_var (CtxU Γ G) i Aj)).
-    rewrite H. f_equal.
-    destruct i; auto; simpl.
-    assert (i+2 = S (S i)) by omega; rewrite H0; auto.
-Qed.
-
-
-Lemma find_op_None_switch h i j op:
-  find_op_case h op = None -> find_op_case (h_switch_vars h i j) op = None.
-Proof.
-intro orig. induction h; auto.
-simpl. simpl in *.
-destruct (op==o).
-+ discriminate.
-+ apply IHh. assumption.
-Qed.
-
-Lemma find_op_Some_switch h i j op x_op k_op c_op:
-  find_op_case h op = Some (x_op, k_op, c_op) ->
-  find_op_case (h_switch_vars h i j) op
-    =
-  Some (x_op, k_op, c_switch_vars c_op (i+2) (j+2)).
-Proof.
-intro orig.
-induction h; auto; simpl; simpl in *.
-+ discriminate.
-+ destruct (op==o).
-  - f_equal. inv orig. auto.
-  - apply IHh. auto.
-Qed.
-
-Lemma v_no_var_j_switch_i_j v i j:
-  v_no_var_j v j -> v_no_var_j (v_switch_vars v j i) i
-with c_no_var_j_switch_i_j c i j:
-  c_no_var_j c j -> c_no_var_j (c_switch_vars c j i) i
-with h_no_var_j_switch_i_j h i j:
-  h_no_var_j h j -> h_no_var_j (h_switch_vars h j i) i.
-Proof.
-{
-clear v_no_var_j_switch_i_j.
-revert i j; induction v; intros i j orig; simpl; auto;
-try constructor; try destruct orig; simpl; auto.
-destruct v as (name, num).
-destruct (num=?j) eqn:cmpj.
-+ simpl in orig. destruct orig. apply Nat.eqb_eq in cmpj. auto.
-+ destruct (num=?i) eqn:cmpi; simpl.
-  * apply Nat.eqb_eq in cmpi. rewrite cmpi in *. simpl in orig. auto.
-  * apply Nat.eqb_neq in cmpi. auto.
-}{
-clear c_no_var_j_switch_i_j.
-revert i j; induction c; intros i j orig; try destruct p; simpl; auto;
-try constructor; try destruct orig; simpl; auto.
-constructor; destruct H0; auto.
-}{
-clear h_no_var_j_switch_i_j.
-revert i j; induction h; intros i j orig; simpl; auto;
-try constructor; try destruct orig; simpl; auto.
-}
-Qed.
 
 Lemma get_ctx_remove_unchanged Γ i j :
   i > j -> get_vtype Γ j = get_vtype (ctx_remove_var Γ i) j.
@@ -255,6 +16,7 @@ destruct i; destruct j; simpl.
 + reflexivity.
 + apply IHΓ. omega.
 Qed.
+
 
 Lemma get_ctx_remove_changed Γ i j :
   i <= j -> get_vtype Γ (S j) = get_vtype (ctx_remove_var Γ i) j.
@@ -268,9 +30,7 @@ Qed.
 Lemma ctx_remove_extend Γ i A :
   CtxU (ctx_remove_var Γ i) A = ctx_remove_var (CtxU Γ A) (i+1).
 Proof.
-revert i; induction Γ; intros i; assert (i+1 = S i) by omega; rewrite H.
-+ reflexivity.
-+ simpl. reflexivity.
+revert i; induction Γ; intros i; assert (i+1 = S i) by omega; rewrite H; auto.
 Qed.
 
 Lemma get_ctx_insert_unchanged Γ A i j:
@@ -299,7 +59,5 @@ Qed.
 Lemma ctx_insert_extend Γ i A_ins A :
   CtxU (ctx_insert_var Γ A_ins i) A = ctx_insert_var (CtxU Γ A) A_ins (i+1).
 Proof.
-revert i; induction Γ; intros i; assert (i+1 = S i) by omega; rewrite H.
-+ reflexivity.
-+ simpl. reflexivity.
+revert i; induction Γ; intros i; assert (i+1 = S i) by omega; rewrite H; auto.
 Qed.
